Modified liveness proof with new assumption and different structure

Graphiti/Projects/Liveness/ComposedLiveness.lean
@@ -10,7 +10,6 @@ import Graphiti.Projects.Liveness.ComposedModule
 import Graphiti.Projects.Liveness.StateTransitionLiveness
 import Graphiti.Core.Trace
 
-
 -- general liveness theorem sketch, as described in "Defining Liveness" paper
 -- (∀α: α ∈ S* : (∃β : β ∈ Sω : αβ respects P))
 -- theorem liveness (P : Trace → Prop)  :
@@ -20,166 +19,6 @@ import Graphiti.Core.Trace
 
 open Graphiti
 open Graphiti.Module
--- namespace Module
--- namespace NatModule
-
--- #check NatModule.gfmodule
-
--- if `f(x)` is in the module, then it can be output (through steps `t'`, leading to new state `s'` which is empty)
-/-
-lemma gcompf_flushability {T} (f g: T → T):
-  ∀ (x: T) (s: State _ _), s.module = (NatModule.gcompf T f g) ∧ (f x) ∈ s.state.fst
-  → ∃ t' s', (@star _ _ (state_transition s.module) ⟨s.state,  s.module⟩ t' ⟨s', s.module⟩)
-  ∧ .output 0 ⟨ T, g (f x) ⟩ ∈ t'
-  ∧ s' = (∅, ∅) := by
-    intros x s h
-    have ⟨ h1, h2 ⟩ := h
-    -- step internal, get s2 with internal state (∅, ∀x∈s -> g(f(x)))
-    have h_int: ∃ s2, step s [] ⟨s2, s.module⟩ := by rw [h1]; sorry -- use h2
-    -- step output
-    have h_out: ∃ s3 v', step s [.output 0 v'] ⟨s3, s.module⟩ := by sorry
-    -- gotta prove that v' = g(f(x)) and that s3 = s'
-    sorry
-
-
-lemma gcompfp_lemma2 {t t': Trace Nat} {T f g} : -- rename it to `gcompf_stuck_input` ?
-  ∀ x (s: State _ _) s', s.module = (NatModule.gcompf T f g)
-  -- ∧ @reachable _ _ (state_transition s.module) t' s
-  ∧ @star _ _ (state_transition s.module) s t s'
-  ∧ .input 0 ⟨ T, x ⟩ ∈ t ∧ .output 0 ⟨ T, g (f x) ⟩ ∉ t
-  → (f x) ∈ s.state.fst ∨ g (f x) ∈ s.state.snd := by
-    sorry
-
--- if some input `x` was fed to g∘f module, but output `g(f(x))` is not out, then `x` is currently *in* the module, either in the first list (as `f(x)`) or in the second list (as `g(f(x))`)
-lemma gcompfp_lemma {t t0: Trace Nat} {T f g} : -- rename it to `gcompf_stuck_input` ?
-  ∀ x (s: State _ _) s', @star _ _ (state_transition s.module) s t s'
-  → s.module = (NatModule.gcompf T f g)
-  → @reachable _ _ (state_transition s.module) t0 s
-  → .input 0 ⟨ T, x ⟩ ∈ (t0 ++ t) → .output 0 ⟨ T, g (f x) ⟩ ∉ (t0 ++ t)
-  → (f x) ∈ s.state.fst ∨ g (f x) ∈ s.state.snd := by
-    -- try to get away from beh asap, so you don't have to start at init state which is empty since we can't induct over that
-    intros x s s' h
-    revert x t0
-    generalize heq: state_transition s.module = n at * -- will need to prove that module stays constant (exist lemma)
-    induction h
-    case refl => sorry
-    case step => sorry
-
-
-
-
-
-def gcompf_P {T} (t: Trace Nat)(f g: T → T) : Prop :=
-  ∀ in1, .input 0 ⟨ T, in1 ⟩ ∈ t → .output 0 ⟨ T, g (f (in1)) ⟩ ∈ t
-
---theorem gcompf_inp {T f g} : ∀ t t0 x, .input 0 ⟨T, x ⟩ ∉ t0 ∧ gcompf_P (t ++ t0) f g ∧ ∃ s s0, @star _ _ (state_transition s.module) s t0 s0
---:= by sorry
-
-theorem gcompf_reachness {T f g} : ∀ t s s', @star _ _ (state_transition (NatModule.gcompf T f g)) s t s'
-  → ∀ t0, (∀ x, .input 0 ⟨ T, x ⟩ ∉ t0)
-  → gcompf_P (t ++ t0) f g
-  → ∀ e s'', @star _ _ (state_transition (NatModule.gcompf T f g)) s' [e] s''
-  → ∃ sn tn,gcompf_P (t ++ [e] ++ tn) f g ∧ @star _ _ (state_transition (NatModule.gcompf T f g)) s'' tn sn ∧ ∀ x, .input 0 ⟨T, x ⟩ ∉ tn:= by sorry
-
-
--- if 0 steps holds, if n steps have to check the reachabilty + */// lemmas: is input included, is output included
--- with module gcompf, if "in1" in trace α, then there exist a β where eventually "out1 = g∘f(in1)" in trace αβ
-theorem gcompf_liveness {t : Trace Nat} {T f g} (h_steps: @behaviour _ _ (state_transition (NatModule.gcompf T f g)) t)  :
-  ∃ t', gcompf_P (t ++ t') (f) (g) ∧ @behaviour _ _ (state_transition (NatModule.gcompf T f g)) (t ++ t') ∧ ∀ x, .input 0 ⟨T, x⟩ ∉ t' := by
-    cases h_steps
-    rename_i s1 behUnfolded
-    have helpNext := (s1.module.state_transition = (state_transition (NatModule.gcompf T f g)))
-    cases behUnfolded
-    rename_i s2 behUnfolded
-    have starRevConv := (@star_eq_star_rev _ _ (state_transition (NatModule.gcompf T f g)) s1 s2 t).mp behUnfolded.right
-    induction starRevConv
-    . exists []
-      simp [gcompf_P]
-      exists s1
-      exists s1
-    . rename_i s3 s4 l1 l2 stepP starP iH
-      have starConv := (@star_eq_star_rev _ _ (state_transition (NatModule.gcompf T f g)) s1 s3 l1).mpr starP
-      have iHEval := iH (And.intro behUnfolded.left starConv)
-      cases iHEval
-      clear iH
-      rename_i l2 iH
-      have stepPP := stepP
-      cases stepP
-      . rename_i ip LxL firstInputV firstInputTpe secondInputV firstInputEq
-        have behConv := iH.right.left
-        simp [behaviour_tight] at behConv
-        cases behConv
-        rename_i s4 behConv
-        cases behConv
-        rename_i s5 behConv
-        cases behConv
-        rename_i stateInits5 cc
-        have lemmaUse :=  @gcompf_reachness T f g
-        simp [reachable] at lemmaUse
-        have stepToStar := @star.plus_one _ _ (state_transition (NatModule.gcompf T f g)) s3 ({ state := LxL, module := s3.module }) ([IOEvent.input ip firstInputTpe]) stepPP
-        have lemmaUse1 := lemmaUse l1 s1 s3 starConv l2 iH.right.right iH.left (IOEvent.input ip firstInputTpe) ({ state := LxL, module := s3.module }) stepToStar
-        cases lemmaUse1
-        rename_i s6 lemma1
-        cases lemma1
-        rename_i l3 indLemma
-        exists l3
-        constructor
-        . simp at *
-          exact indLemma.left
-        . constructor
-          . simp [behaviour]
-            exists s1
-            constructor
-            . exact behUnfolded.left
-            . clear lemmaUse
-              exists s6
-              have firstSteps := @star.trans_star _ _ (state_transition (NatModule.gcompf T f g)) s1 s3 ({ state := LxL, module := s3.module }) l1 [IOEvent.input ip firstInputTpe] starConv
-              have firstSteps1 := firstSteps stepToStar
-              have secondSteps := @star.trans_star _ _ (state_transition (NatModule.gcompf T f g)) s1 { state := LxL, module := s3.module } s6 (l1 ++ [IOEvent.input ip firstInputTpe]) l3 firstSteps1 indLemma.right.left
-              simp at *
-              assumption
-          . exact indLemma.right.right
-      . rename_i ip LxL firstInputV firstInputTpe secondInputV firstInputEq
-        have behConv := iH.right.left
-        simp [behaviour_tight] at behConv
-        cases behConv
-        rename_i s4 behConv
-        cases behConv
-        rename_i s5 behConv
-        cases behConv
-        rename_i stateInits5 cc
-        have lemmaUse :=  @gcompf_reachness T f g
-        simp [reachable] at lemmaUse
-        have stepToStar := @star.plus_one _ _ (state_transition (NatModule.gcompf T f g)) s3 ({ state := LxL, module := s3.module }) ([IOEvent.output ip firstInputTpe]) stepPP
-        have lemmaUse1 := lemmaUse l1 s1 s3 starConv l2 iH.right.right iH.left (IOEvent.output ip firstInputTpe) ({ state := LxL, module := s3.module }) stepToStar
-        cases lemmaUse1
-        rename_i s6 lemma1
-        cases lemma1
-        rename_i l3 indLemma
-        exists l3
-        constructor
-        . simp at *
-          exact indLemma.left
-        . constructor
-          . simp [behaviour]
-            exists s1
-            constructor
-            . exact behUnfolded.left
-            . clear lemmaUse
-              exists s6
-              have firstSteps := @star.trans_star _ _ (state_transition (NatModule.gcompf T f g)) s1 s3 ({ state := LxL, module := s3.module }) l1 [IOEvent.output ip firstInputTpe] starConv
-              have firstSteps1 := firstSteps stepToStar
-              have secondSteps := @star.trans_star _ _ (state_transition (NatModule.gcompf T f g)) s1 { state := LxL, module := s3.module } s6 (l1 ++ [IOEvent.output ip firstInputTpe]) l3 firstSteps1 indLemma.right.left
-              simp at *
-              assumption
-          . exact indLemma.right.right
-      . rename_i RLL LL RLLInS3 RLLS
-        exists l2
-        simp at *
-        assumption
--/
-
-
 
 /-
 New approach: using behaviours is too limiting, I decided to do a secondary proof exclusively on star and prove behaviour
@@ -194,7 +33,30 @@ theorem gcompf_lemm_in {T f g}: ∀ t0 t s s0 e, (∀ x, .input 0 ⟨T, x⟩ ∉
 → gcompf_P (t ++ t0) f g
 → @star _ _ (state_transition (NatModule.gcompf T f g)) s t0 s0
 → gcompf_P (t ++ [.input 0 ⟨T, e⟩  ] ++ t0 ++ [.output 0 ⟨ T, g (f e) ⟩ ]) f g
-:= by sorry
+:= by
+  intro t0 t s s0 e prop compPrev star
+  simp [gcompf_P] at *
+  simp [prop] at compPrev
+  intro in1 assum
+  cases assum
+  . rename_i p1
+    have compEval := compPrev in1 p1
+    cases compEval
+    rename_i a
+    left
+    exact a
+    rename_i a
+    right; left
+    exact a
+  . rename_i a
+    cases a
+    rename_i subProp
+    subst subProp
+    right; right
+    simp
+    rename_i abs
+    exfalso
+    simp [prop] at abs
 
 
 
@@ -202,8 +64,9 @@ theorem gcompf_lemm_out {T f g}: ∀ t0 t s s0 e, (∀ x, .input 0 ⟨T, x⟩ �
 → gcompf_P (t ++ t0) f g
 → @star _ _ (state_transition (NatModule.gcompf T f g)) s t0 s0
 → ∃ t0', gcompf_P (t ++ [.output 0 ⟨ T, e ⟩] ++ t0') f g
-∧ t0 = ([.output 0 ⟨ T, e ⟩] ++ t0'):= by sorry
-
+∧ t0 = ([.output 0 ⟨ T, e ⟩] ++ t0'):= by
+  intro t0 t1 s1 s0 e iProp star
+  sorry
 
 
 
@@ -269,30 +132,42 @@ theorem gcompf_reachness_empty {T f g} : ∀ t s', @reachable _ _ (state_transit
 theorem gcompf_reachness_input {T f g} : ∀ t s', @reachable _ _ (state_transition (NatModule.gcompf T f g)) t s'
 → ∀ s'' t0, ( ∀ x, .input 0 ⟨ T, x ⟩ ∉ t0) ∧ @star _ _ (state_transition (NatModule.gcompf T f g)) s' t0 s''
 → gcompf_P (t ++ t0) f g
-→ ∀ n io s''', @step _ _ _ s' [IOEvent.input n io] s'''
-→ ∃ sn tn, gcompf_P (t ++ [IOEvent.input n io] ++ tn) f g ∧ @star _ _ (state_transition (NatModule.gcompf T f g)) s''' tn sn ∧ ∀ x, .input 0 ⟨T, x ⟩ ∉ tn:= by
-  intro l1 s1 reachP s2 l2  noInpiInL2 gcomfProp n io s3 step
+→ ∀ x s''', @step _ _ _ s' [IOEvent.input 0 ⟨T, x⟩] s'''
+→ ∃ sn tn, gcompf_P (t ++ [IOEvent.input 0 ⟨T, x⟩] ++ tn) f g ∧ @star _ _ (state_transition (NatModule.gcompf T f g)) s''' tn sn ∧ ∀ x, .input 0 ⟨T, x ⟩ ∉ tn:= by
+  intro l1 s1 reachP s2 l2  noInpiInL2 gcomfProp io s3 step
   sorry
 
-
-theorem gcompf_reachness_output {T f g} : ∀ t s', @reachable _ _ (state_transition (NatModule.gcompf T f g)) t s'
-→ ∀ s'' t0, ( ∀ x, .input 0 ⟨ T, x ⟩ ∉ t0) ∧ @star _ _ (state_transition (NatModule.gcompf T f g)) s' t0 s''
+/--
+theorem gcompf_reachness_output { T f g} : ∀ t s', @reachable _ _ (state_transition (NatModule.gcompf T f g)) t  ⟨ s', (NatModule.gcompf T f g)⟩
+→ ∀ s'' t0 ,( ∀ x, .input 0 ⟨T, x ⟩ ∉ t0) ∧ @star _ _ (state_transition (NatModule.gcompf T f g)) ⟨ s', (NatModule.gcompf T f g)⟩ t0 s''
 → gcompf_P (t ++ t0) f g
-→ ∀ n io s''', @step _ _ _ s' [IOEvent.output n io] s'''
-→ ∃ sn tn, gcompf_P (t ++ [IOEvent.output n io] ++ tn) f g ∧ @star _ _ (state_transition (NatModule.gcompf T f g)) s''' tn sn ∧ ∀ x, .input 0 ⟨T, x ⟩ ∉ tn:= by
-  intro l1 s1 reachP s2 l2  noInpiInL2 gcomfProp n io s3 step
+→ ∀ io s''', @step _ _ _ ⟨ s', (NatModule.gcompf T f g)⟩ [IOEvent.output 0 ⟨ T, io⟩]  s'''
+→ ∃ sn tn, gcompf_P (t ++ [IOEvent.output 0 ⟨T, io ⟩] ++ tn) f g ∧ @star _ _ (state_transition (NatModule.gcompf T f g)) s''' tn sn ∧ ∀ x, .input 0 ⟨T, x ⟩ ∉ tn:= by
+  intro l1 s1 reachP s2 l2 noInpiInL2 gcomfProp io s3 step
   cases step
-  rename_i state s1Tpe s1Trans s1Eq
-  have use_lemm := @gcompf_lemm_in T f g l2 l1 s1 s2
-  simp [NatModule.gcompf] at *
+  rename_i s' v a a'
+  simp at *
+  rw [PortMap.rw_rule_execution (by simp [drunfold]; rfl)] at *
+  sorry
+-/
+theorem gcompf_reachness_output { T f g} : ∀ t s', @reachable _ _ (state_transition (NatModule.gcompf T f g)) t  s'
+→ ∀ s'' t0 ,( ∀ x, .input 0 ⟨T, x ⟩ ∉ t0) ∧ @star _ _ (state_transition (NatModule.gcompf T f g)) s' t0 s''
+→ gcompf_P (t ++ t0) f g
+→ ∀ io s''', @step _ _ _ s' [IOEvent.output 0 ⟨ T, io⟩]  s'''
+→ ∃ sn tn, gcompf_P (t ++ [IOEvent.output 0 ⟨T, io ⟩] ++ tn) f g ∧ @star _ _ (state_transition (NatModule.gcompf T f g)) s''' tn sn ∧ ∀ x, .input 0 ⟨T, x ⟩ ∉ tn:= by
+  intro l1 s1 reachP s2 l2 noInpiInL2 gcomfProp io s3 step
+  cases step
+  rename_i s' v a a'
+  simp at *
+  rw [PortMap.rw_rule_execution (by simp [drunfold]; rfl)] at *
   sorry
 
 
-
-
-
-
-theorem gcompf_liveness_simp {t : Trace Nat} {T f g} (s1 s2: State _ _) (h: @StateTransition.init _ _ (state_transition (NatModule.gcompf T f g)) s1 ∧ @star _ _ (state_transition (NatModule.gcompf T f g)) s1 t s2):
+theorem gcompf_liveness_simp {t : Trace Nat} {T f g}
+(h_in: (∀ G x n, IOEvent.input n ⟨G, x⟩  ∈ t → (n = 0) ∧ G = T))
+(h_out: (∀ G x n, IOEvent.output n ⟨G, x⟩  ∈ t → (n = 0) ∧ G = T))
+(s1 s2: State _ _)
+(h: @StateTransition.init _ _ (state_transition (NatModule.gcompf T f g)) s1 ∧ @star _ _ (state_transition (NatModule.gcompf T f g)) s1 t s2):
   ∃ t' s3, gcompf_P (t ++ t') f g ∧ @star _ _ (state_transition (NatModule.gcompf T f g)) s2 t' s3 ∧ (∀ x, .input 0 ⟨T, x⟩ ∉ t'):= by
     have starConv := (@star_eq_star_rev _ _ (state_transition (NatModule.gcompf T f g)) s1 s2 t).mp h.right
     induction starConv
@@ -303,7 +178,22 @@ theorem gcompf_liveness_simp {t : Trace Nat} {T f g} (s1 s2: State _ _) (h: @Sta
     . rename_i s3 s4 l1 l2 step star iH
       have starConv := (@star_eq_star_rev _ _ (state_transition (NatModule.gcompf T f g)) s1 s3 l1).mpr star
       clear star
-      have iHRes := iH (And.intro h.left starConv)
+      simp at h_in h_out
+      have h_in_new : (∀ (G : Type) (x : G) (n : InternalPort ℕ), IOEvent.input n ⟨G, x⟩ ∈ l1 → n = 0 ∧ G = T) := by {
+        intro G x n exp
+        have h_in_up := h_in G x n
+        apply h_in_up
+        constructor
+        assumption
+      }
+      have h_out_new : (∀ (G : Type) (x : G) (n : InternalPort ℕ), IOEvent.output n ⟨G, x⟩ ∈ l1 → n = 0 ∧ G = T) := by {
+        intro G x n exp
+        have h_out_up := h_out G x n
+        apply h_out_up
+        constructor
+        assumption
+      }
+      have iHRes := iH h_in_new h_out_new (And.intro h.left starConv)
       clear iH
       cases iHRes
       rename_i tr iH
@@ -314,9 +204,16 @@ theorem gcompf_liveness_simp {t : Trace Nat} {T f g} (s1 s2: State _ _) (h: @Sta
       . rename_i IntN LTPair s3Fst TT s3Snd TTEq
         have finalRes := @gcompf_reachness_input T f g l1 s3
         simp [reachable] at finalRes
-        have finalResT := finalRes s1 h.left starConv s5 tr iH.right.right iH.right.left iH.left IntN TT
+        have finalResT := finalRes s1 h.left starConv s5 tr iH.right.right iH.right.left iH.left
+        cases TT
+        rename_i TT inp
+        have h_in_assum := h_in TT inp IntN
+        simp at h_in_assum
         clear finalRes
-        have finalRes := finalResT { state := LTPair, module := s3.module } keepStep
+        rcases h_in_assum with ⟨ nEq, TypeEq ⟩
+        subst nEq
+        subst TypeEq
+        have finalRes := finalResT inp { state := LTPair, module := s3.module } keepStep
         cases finalRes
         rename_i s4 finalRes
         cases finalRes
@@ -328,10 +225,16 @@ theorem gcompf_liveness_simp {t : Trace Nat} {T f g} (s1 s2: State _ _) (h: @Sta
       . rename_i IntN LTPair s3Fst TT s3Snd TTEq
         have finalRes :=@ gcompf_reachness_output T f g l1 s3
         simp [reachable] at finalRes
-        have finalResT := finalRes s1 h.left starConv s5 tr iH.right.right iH.right.left iH.left IntN TT
+        have finalResT := finalRes s1 h.left starConv s5 tr iH.right.right iH.right.left iH.left
+        cases TT
+        rename_i TT inp
+        have h_out_assum := h_out TT inp IntN
+        simp at h_out_assum
         clear finalRes
-        have stepToStar := @star.plus_one _ _ (state_transition (NatModule.gcompf T f g)) s3 ({ state := LTPair, module := s3.module }) [IOEvent.output IntN TT]
-        have finalRes := finalResT { state := LTPair, module := s3.module } keepStep
+        rcases h_out_assum with ⟨ nEq, TypeEq ⟩
+        subst nEq
+        subst TypeEq
+        have finalRes := finalResT inp { state := LTPair, module := s3.module } keepStep
         cases finalRes
         rename_i s4 finalRes
         cases finalRes
@@ -358,7 +261,9 @@ theorem gcompf_liveness_simp {t : Trace Nat} {T f g} (s1 s2: State _ _) (h: @Sta
 
 
 
-theorem gcompf_liveness2 {t : Trace Nat} {T f g} (h_steps: @behaviour _ _ (state_transition (NatModule.gcompf T f g)) t)  :
+theorem gcompf_liveness2 {t : Trace Nat} {T f g}(h_steps: @behaviour _ _ (state_transition (NatModule.gcompf T f g)) t)
+(h_in: (∀ G x n, IOEvent.input n ⟨G, x⟩  ∈ t → (n = 0) ∧ G = T))
+(h_out: (∀ G x n, IOEvent.output n ⟨G, x⟩  ∈ t → (n = 0) ∧ G = T)):
   ∃ t', gcompf_P (t ++ t') (f) (g) ∧ @behaviour _ _ (state_transition (NatModule.gcompf T f g)) (t ++ t') ∧ ∀ x, .input 0 ⟨T, x⟩ ∉ t' := by
     simp [behaviour] at h_steps
     cases h_steps
@@ -367,7 +272,7 @@ theorem gcompf_liveness2 {t : Trace Nat} {T f g} (h_steps: @behaviour _ _ (state
     rename_i p1 beh
     cases beh
     rename_i s2 star
-    have mainProof := gcompf_liveness_simp s1 s2 (And.intro p1 star)
+    have mainProof := gcompf_liveness_simp h_in h_out s1 s2 (And.intro p1 star)
     cases mainProof
     rename_i t' mainProof
     cases mainProof
